\section{Multilayer Perceptrons}
\label{sec:mlp}

\begin{frame}
  \begin{center}
    \Huge{\textcolor{red}{Multilayer Perceptrons}}
  \end{center}
\end{frame}

\subsection{MLP}

\begin{frame}{符号}
 \begin{itemize}
   \item \alert{$ {n_{\ell}} $}: 网络层数，其中第$0$层为输入层，第$n_{\ell}$层为输出层
   \item \alert{$ {s_{\ell}} $}: 第$\ell$层的节点数，$ \ell = 0, 1, ..., n_{\ell} $
   \item \alert{$ w_{ji}^{(\ell)} $}: 第$(\ell-1)$层节点$i$与第$\ell$层节点$j$之间的权重，$ \ell = 1, ..., n_{\ell} $
   \item \alert{$ b_i^{(\ell)} $}: 第$\ell$层节点$i$的偏置项，$ \ell = 1, ..., n_{\ell} $
   \item \alert{$ a_i^{(\ell)} $}: 第$\ell$层节点$i$的输出，$ \ell = 1, ..., n_{\ell}, x = a^{(0)}, y = a^{(n_{\ell})} $
   \item \alert{$ z_i^{(\ell)} $}: 第$\ell$层节点$i$的权重和，$ \ell = 1, ..., n_{\ell} $
   \item \alert{$ \delta _i^{(\ell)} $}: 第$\ell$层节点$i$的误差项，$ \ell = 1, ..., n_{\ell} $
   \item \alert{$ S = \{ ({x^{(t)}},{y^{(t)}});t = 1,2,...,m\} $}: 样本空间
 \end{itemize}
\end{frame}

\begin{frame}{目标函数}
\begin{block}{单个样本}
\[J(w,b;x,y) = \frac{1}{2}{\left( {{h_{w,b}}(x,y) - y} \right)^2}\]
\end{block}

\begin{block}{$m$个样本}
\[J(w,b) = \frac{1}{m}\sum\limits_{t = 1}^m {J\left( {w,b;{x^{(t)}},{y^{(t)}}} \right)} \]
\end{block}

\begin{block}{正则化}
\[J(w,b) = \frac{1}{m}\sum\limits_{t = 1}^m {J\left( {w,b;{x^{(t)}},{y^{(t)}}} \right)}  + \frac{\lambda }{2}\sum\limits_{\ell  = 1}^{{n_\ell }} {\sum\limits_{i = 1}^{{s_{\ell  - 1}}} {\sum\limits_{j = 1}^{{s_\ell }} {{{\left( {w_{ji}^{(\ell )}} \right)}^2}} } } \]
\end{block}
\end{frame}

\begin{frame}{前向输出}
  \begin{figure}
    \centering
    \includegraphics[width=0.75\textwidth]{mlp-forward.png}
  \end{figure}
\end{frame}

\begin{frame}{前向输出}
\begin{block}{向量}
\[\begin{gathered}
  {z^{(\ell )}} = {w^{(\ell )}}{a^{(\ell  - 1)}} + {b^{(\ell )}} \hfill \\
  {a^{(\ell )}} = f({z^{(\ell )}}) \hfill \\
  {a^{(0)}} = x \quad y = {a^{({n_\ell })}} \hfill \\ 
\end{gathered} \]
\end{block}

\begin{block}{标量}
\[\begin{gathered}
  z_i^{(\ell )} = \sum\limits_{h = 1}^{{s_{\ell  - 1}}} {\left( {w_{ih}^{(\ell )}a_h^{(\ell  - 1)} + b_i^{(\ell )}} \right)}  \hfill \\
  a_i^{(\ell )} = f\left( {z_i^{(\ell )}} \right) \hfill \\
  i = 1,2,...,{s_\ell } \quad \ell  = 1,2,...,{n_\ell } \hfill \\ 
\end{gathered} \]
\end{block}
\end{frame}

\begin{frame}{反向传播}
  \begin{figure}
    \centering
    \includegraphics[width=0.45\textwidth]{mlp-backward.png}
  \end{figure}
\end{frame}

\begin{frame}{反向传播}
\begin{block}{向量}
\[{\delta ^{(\ell)}} = \left\{ \begin{gathered}
  {({w^{(\ell + 1)}})^T}{\delta ^{(\ell + 1)}} \circ f\,'({z^{(\ell)}});{\text{  }}\ell \ne {n_\ell} \hfill \\
  ({a^{(\ell)}} - y) \circ f\,'({z^{(\ell)}}); {\text{  }}\ell = {n_\ell} \hfill \\ 
\end{gathered}  \right.\]
\end{block}

\begin{block}{标量}
\[\begin{gathered}
  \delta _i^{(\ell )} = \left\{ \begin{gathered}
  f\,'\left( {z_i^{(\ell )}} \right)\sum\limits_{j = 1}^{{s_{\ell  + 1}}} {w_{ji}^{(\ell  + 1)}\delta _j^{(\ell  + 1)}} {\text{   }}\ell  \ne {n_\ell } \hfill \\
  f\,'\left( {z_i^{(\ell )}} \right)\left( {a_i^{(\ell )} - {y_i}} \right){\text{       }}\ell  = {n_\ell } \hfill \\ 
\end{gathered}  \right. \hfill \\
  i = 1,2,...,{s_\ell } \hfill \\ 
\end{gathered} \]
\end{block}
\end{frame}

\begin{frame}{梯度计算}
  \begin{figure}
    \centering
    \includegraphics[width=0.5\textwidth]{mlp-grad.png}
  \end{figure}
\end{frame}

\begin{frame}{梯度计算}
\begin{block}{向量}
\[\begin{gathered}
  {\nabla _{{w^{(\ell )}}}}J(w,b;x,y) = {\delta ^{(\ell )}}{\left( {{a^{(\ell  - 1)}}} \right)^T} \hfill \\
  {\nabla _{{b^{(\ell )}}}}J(w,b;x,y) = {\delta ^{(\ell )}} \hfill \\
  \ell  = 1,2,...,{n_\ell } \hfill \\ 
\end{gathered} \]
\end{block}

\begin{block}{标量}
\[\begin{gathered}
  {\nabla _{w_{ih}^{(\ell )}}}J(w,b;x,y) = \delta _i^\ell a_h^{(\ell  - 1)} \hfill \\
  {\nabla _{b_i^{(\ell )}}}J(w,b;x,y) = \delta _i^\ell  \hfill \\
  i = 1,2,...,{s_\ell } \quad \ell  = 1,2,...,{n_\ell } \hfill \\ 
\end{gathered} \]
\end{block}
\end{frame}

\begin{frame}{变化量}
\begin{block}{向量}
\[\begin{aligned}
  \Delta {w^{(\ell )}} \leftarrow \Delta {w^{(\ell )}} + {\nabla _{{w^{(\ell )}}}}J\left( {w,b;{x^{(t)}},{y^{(t)}}} \right) \\ 
  \Delta {b^{(\ell )}} \leftarrow \Delta {b^{(\ell )}} + {\nabla _{{b^{(\ell )}}}}J\left( {w,b;{x^{(t)}},{y^{(t)}}} \right) \\ 
  t = 1,2,...,m;\ell  = 1,2,...,{n_\ell } \\ 
\end{aligned} \]
\end{block}

\begin{block}{标量}
\[\begin{gathered}
  \Delta w_{ih}^{(\ell )} \leftarrow \Delta w_{ih}^{(\ell )} + {\nabla _{w_{ih}^{(\ell )}}}J\left( {w,b;{x^{(t)}},{y^{(t)}}} \right) \hfill \\
  \Delta b_i^{(\ell )} \leftarrow \Delta b_i^{(\ell )} + {\nabla _{b_i^{(\ell )}}}J\left( {w,b;{x^{(t)}},{y^{(t)}}} \right) \hfill \\
  t = 1,2,...,m;\ell  = 1,2,...,{n_\ell };i = 1,2,...,{s_\ell };h = 1,2,...,{s_{\ell  - 1}} \hfill \\ 
\end{gathered} \]
\end{block}
\end{frame}

\begin{frame}{权重更新}

\begin{block}{向量}
\[\begin{aligned}
  {w^{(\ell )}} \leftarrow  & {w^{(\ell )}} - \alpha \left( {\frac{{\Delta {w^{(\ell )}}}}{m}} \right) \\ 
  {b^{(\ell )}} \leftarrow  & {b^{(\ell )}} - \alpha \frac{{\Delta {b^{(\ell )}}}}{m} \\ 
  \ell  = & 1,2,...,{n_\ell }  \\
\end{aligned} \]
\end{block}

\begin{block}{正则项}
\[\begin{aligned}
  {w^{(\ell )}} \leftarrow  & {w^{(\ell )}} - \alpha \left( {\frac{{\Delta {w^{(\ell )}}}}{m} + \lambda {w^{(\ell )}}} \right) \\ 
\end{aligned} \]
\end{block}
\end{frame}


\begin{frame}{权重更新}

\begin{block}{标量}
\[\begin{gathered}
  w_{ih}^{(\ell )} \leftarrow w_{ih}^{(\ell )} - \alpha \frac{{\Delta w_{ih}^{(\ell )}}}{m} \hfill \\
  b_i^{(\ell )} \leftarrow b_i^{(\ell )} - \alpha \frac{{\Delta b_i^{(\ell )}}}{m} \hfill \\
  \ell  = 1,2,...,{n_\ell };i = 1,2,...,{s_\ell };h = 1,2,...,{s_{\ell  - 1}} \hfill \\ 
\end{gathered} \]
\end{block}

\begin{block}{正则项}
\[\begin{gathered}
  w_{ih}^{(\ell )} \leftarrow w_{ih}^{(\ell )} - \alpha \left( {\frac{{\Delta w_{ih}^{(\ell )}}}{m} + \lambda w_{ih}^{(\ell )}} \right) \hfill \\
  \ell  = 1,2,...,{n_\ell };i = 1,2,...,{s_\ell };h = 1,2,...,{s_{\ell  - 1}} \hfill \\ 
\end{gathered} \]
\end{block}

\end{frame}
